Semantics/Imp/Bexp.lean
@@ -7,13 +7,17 @@ namespace Natural
 inductive step: Bexp → State → Bool → Prop
   | tt: step tt _ true
   | ff: step ff _ false
-  | le: step (le a b) s (a⇓s ≤ b⇓s)
   | not
     (h: step a s n):
     step (not a) s (!n)
   | and
     (h₁: step a s n) (h₂: step b s m):
     step (and a b) s (n && m)
+  | or
+    (h₁: step a s n) (h₂: step b s m):
+    step (or a b) s (n || m)
+  | eq: step (eq a b) s (a⇓s = b⇓s)
+  | le: step (le a b) s (a⇓s ≤ b⇓s)
 
 notation s " ⊢ " a " ⟹ " v => step a s v
 
@@ -26,6 +30,8 @@ end Natural
   | ff      => false
   | not b   => !reduce b s
   | and a b => reduce a s && reduce b s
+  | or a b => reduce a s || reduce b s
+  | eq a b  => a.reduce s = b.reduce s
   | le a b  => a.reduce s ≤ b.reduce s
 
 infix:100 "⇓" => reduce
@@ -35,14 +41,17 @@ theorem Natural.from_reduce {b: Bexp} (h: b⇓s = x): s ⊢ b ⟹ x :=
   by induction b generalizing x with
   | tt => exact h ▸ step.tt
   | ff => exact h ▸ step.ff
-  | le => exact h ▸ step.le
   | not _ ih => exact h ▸ step.not (ih rfl)
   | and _ _ l r => exact h ▸ step.and (l rfl) (r rfl)
+  | or _ _ l r => exact h ▸ step.or (l rfl) (r rfl)
+  | eq => exact h ▸ step.eq
+  | le => exact h ▸ step.le
 
 theorem reduce.from_natural {b: Bexp} (h: s ⊢ b ⟹ x): b⇓s = x :=
   by induction h with
   | not _ ih => exact ih ▸ rfl
   | and _ _ ih₁ ih₂ => exact ih₁ ▸ ih₂ ▸ rfl
+  | or _ _ ih₁ ih₂ => exact ih₁ ▸ ih₂ ▸ rfl
   | _ => rfl
 
 @[simp] theorem step_eq_reduce {b: Bexp}: (s ⊢ b ⟹ x) ↔ b⇓s = x := ⟨reduce.from_natural, Natural.from_reduce⟩
